WIP:Prove real-valued simulation, start drafting floating-point simulation

icing/CakeMLtoFloVerProofsScript.sml
@@ -1,14 +1,81 @@
 (* HOL4 *)
 open machine_ieeeTheory realTheory realLib RealArith;
 (* CakeML *)
-open compilerTheory;
+open semanticPrimitivesTheory terminationTheory compilerTheory;
 (* FloVer *)
-open ExpressionsTheory CommandsTheory IEEE_connectionTheory;
+open ExpressionsTheory ExpressionSemanticsTheory CommandsTheory
+     EnvironmentsTheory IEEE_connectionTheory
+     FloverMapTheory TypeValidatorTheory;
 (* Icing *)
-open CakeMLtoFloVerTheory;
+open CakeMLtoFloVerTheory CakeMLtoFloVerLemsTheory;
 open preamble;
 
 val _ = new_theory "CakeMLtoFloVerProofs";
+
+(* TODO: Move to HOL4 distrib *)
+Theorem float_is_finite_sandwich:
+  ∀ (w1:('a,'b) float) (w2:('a,'b) float) (w3:('a,'b) float).
+  float_less_equal w1 w2 ∧
+  float_less_equal w2 w3 ∧
+  float_is_finite w1 ∧
+  float_is_finite w3 ⇒
+  float_is_finite w2
+Proof
+  rpt strip_tac
+  \\ fs[binary_ieeeTheory.float_is_finite_def,
+        binary_ieeeTheory.float_less_equal_def]
+  \\ Cases_on ‘float_value w1’ \\ fs[]
+  \\ Cases_on ‘float_value w3’ \\ fs[]
+  \\ Cases_on ‘float_compare w1 w2’ \\ fs[]
+  \\ Cases_on ‘float_compare w2 w3’ \\ rfs[binary_ieeeTheory.float_compare_def]
+  \\ Cases_on ‘float_value w2’ \\ fs[]
+  \\ Cases_on ‘w2.Sign = 1w’ \\ fs[]
+QED
+
+Theorem fp64_isFinite_sandwich:
+  ∀ w1 w2 w3.
+    fp64_lessEqual w1 w2 ∧
+    fp64_lessEqual w2 w3 ∧
+    fp64_isFinite w1 ∧
+    fp64_isFinite w3 ⇒
+    fp64_isFinite w2
+Proof
+  fs[fp64_lessEqual_def, fp64_isFinite_def]
+  \\ rpt strip_tac
+  \\ irule float_is_finite_sandwich
+  \\ fsrw_tac [SATISFY_ss] []
+QED
+
+Theorem closest_such_0:
+  ∀ (f:('a, 'b) float).
+  closest_such (λ a. ~word_lsb a.Significand) float_is_finite 0 = f ⇒
+  f = float_plus_zero (:'a # 'b) ∨ f = float_minus_zero (:'a # 'b)
+Proof
+  rpt strip_tac \\ rveq
+  \\ fs[binary_ieeeTheory.closest_such_def]
+  \\ SELECT_ELIM_TAC \\ rpt strip_tac
+  >- (
+    fs[binary_ieeeTheory.is_closest_def]
+    \\ qexists_tac ‘float_plus_zero (:'a # 'b)’
+    \\ fs[binary_ieeeTheory.float_is_finite, IN_DEF,
+          binary_ieeeTheory.zero_properties, binary_ieeeTheory.zero_to_real,
+          ABS_POS]
+    \\ rpt strip_tac
+    \\ fs[wordsTheory.word_lsb_def, binary_ieeeTheory.float_plus_zero_def]
+    \\ pop_assum (fn thm => assume_tac (EVAL_RULE thm)) \\ fs[])
+  \\ fs[binary_ieeeTheory.is_closest_def]
+  \\ last_x_assum (qspec_then ‘float_plus_zero (:'a # 'b)’ mp_tac)
+  \\ simp[binary_ieeeTheory.float_is_finite, IN_DEF,
+          binary_ieeeTheory.zero_properties, binary_ieeeTheory.zero_to_real,
+          ABS_POS]
+  \\ rpt strip_tac
+  \\ ‘float_is_zero x’ by (fs[binary_ieeeTheory.float_is_zero_to_real])
+  \\ fs[binary_ieeeTheory.float_is_zero, binary_ieeeTheory.float_plus_zero_def,
+        binary_ieeeTheory.float_minus_zero_def]
+  \\ Cases_on ‘x’ \\ Cases_on ‘c’ \\ Cases_on ‘n’ \\ fs[]
+  \\ TRY (rename1 ‘SUC n < 2’ \\ Cases_on ‘n’)
+  \\ fs[binary_ieeeTheory.float_negate_def, binary_ieeeTheory.float_component_equality]
+QED
 
 Theorem isFloVerExps_toFloVerExp_succeeds:
   ∀ es.
@@ -46,27 +113,7 @@ Proof
   \\ last_x_assum (qspecl_then [‘ids3’, ‘freshId3’] assume_tac) \\ fs[]
 QED
 
-Theorem toFloVerExp_usedVars:
-  ∀ ids freshId e ids2 freshId2 fexp.
-    toFloVerExp ids freshId e = SOME (ids2, freshId2, fexp) ⇒
-    ∀ n. freshId ≤ n ∧ n < freshId2 ⇒
-      n IN domain (usedVars (fexp))
-Proof
-  ho_match_mp_tac toFloVerExp_ind
-  \\ rpt strip_tac \\ fs[toFloVerExp_def]
-  >- (
-   qpat_x_assum ‘_ = SOME _’ mp_tac
-   \\ rpt (TOP_CASE_TAC \\ fs[])
-   \\ rpt strip_tac \\ rveq \\ fs[usedVars_def])
-  \\ qpat_x_assum ‘_ = SOME _’ mp_tac
-  \\ rpt (TOP_CASE_TAC \\ fs[])
-  \\ rpt strip_tac \\ rveq \\ simp[Once usedVars_def, domain_union]
-  \\ TRY (metis_tac[])
-  \\ TRY (Cases_on ‘n < q'’\\ fs[] \\ metis_tac[])
-  \\ TRY (Cases_on ‘n < q'’\\ fs[] \\ TRY (metis_tac[])
-          \\ Cases_on ‘n < q'3'’ \\ fs[] \\ metis_tac[])
-QED
-
+(*
 Theorem isFloVerCmd_toFloVerCmd_succeeds:
   ∀ e ids freshId.
     isFloVerCmd e ⇒
@@ -89,128 +136,7 @@ Proof
   \\ rename1 ‘lookupCMLVar x ids = SOME v’
   \\ Cases_on ‘v’ \\ fs[]
 QED
-
-Definition freevars_def:
-  freevars [] = EMPTY ∧
-  freevars [ast$Var n] = { n } ∧
-  freevars [Lit l] = EMPTY ∧
-  freevars [Raise e] = freevars [e] ∧
-  freevars [Handle e pes] =
-    FOLDL (λ vars. λ (p,e). (freevars [e]) ∪ vars) (freevars [e]) pes ∧
-  freevars [Con id es] = freevars es ∧
-  freevars [Fun s e] = freevars [e] DIFF { Short s } ∧
-  freevars [App op es] = freevars es ∧
-  freevars [Log lop e1 e2] = (freevars [e1] ∪ freevars [e2]) ∧
-  freevars [If e1 e2 e3] = (freevars [e1] ∪ freevars [e2] ∪ freevars [e3]) ∧
-  freevars [Mat e pes] =
-    FOLDL (λ vars. λ (p,e). (freevars [e]) ∪ vars) (freevars [e]) pes ∧
-  freevars [Let x e1 e2] =
-    freevars [e1] ∪
-    (freevars [e2] DIFF (case x of | NONE => EMPTY | SOME s => { Short s })) ∧
-  freevars [Letrec fs e] = EMPTY (* TODO *) ∧
-  freevars [Tannot e t] = freevars [e] ∧
-  freevars [Lannot e l] = freevars [e] ∧
-  freevars [FpOptimise opt e] = freevars [e] ∧
-  freevars (e1::es) =
-    freevars [e1] ∪ freevars es
-Termination
-  wf_rel_tac ‘measure exp6_size’ \\ fs[]
-  \\ Induct_on ‘pes’ \\ fs[]
-  \\ rpt strip_tac \\ simp[astTheory.exp_size_def]  \\ rveq
-  \\ res_tac
-  >- (simp[astTheory.exp_size_def])
-  \\ first_x_assum (qspec_then ‘e’ assume_tac) \\ fs[]
-End
-
-Theorem lookupCMLVar_id_l:
-  lookupCMLVar x ids = SOME (y, n) ⇒
-  x = y
-Proof
-  Induct_on ‘ids’ \\ fs[lookupCMLVar_def, updateTheory.FIND_def]
-  \\ strip_tac \\ rename1 ‘(λ (m,i). x = m) h’ \\ Cases_on ‘h’ \\  fs[]
-  \\ TOP_CASE_TAC \\ fs[]
-QED
-
-Theorem getInterval_inv:
-  getInterval e = SOME (x,lo,hi) ⇒
-  freevars [e] = { Short x } ∧
-  ∃ w1 w2.
-  e = Log And (App (FP_cmp FP_LessEqual) [Lit (Word64 w1); Var (Short x)])
-  (App (FP_cmp FP_LessEqual) [Var (Short x); Lit (Word64 w2)]) ∧
-  lo = fp64_to_real w1 ∧
-  hi = fp64_to_real w2 ∧
-  fp64_isFinite w1 ∧
-  fp64_isFinite w2
-Proof
-  Cases_on ‘e’ \\ simp[getInterval_def]
-  \\ rpt (TOP_CASE_TAC \\ fs[])
-  \\ rpt strip_tac \\ rveq \\ fs[freevars_def]
-QED
-
-Theorem toFloVerPre_freevar_FIND:
-  ∀ cake_P ids floverP dVars.
-  toFloVerPre cake_P ids = SOME (floverP, dVars) ⇒
-  ∀ x. x IN freevars cake_P ⇒
-  ∃ n m. lookupCMLVar x ids = SOME (x, n) ∧
-  FIND (λ m. n = m) dVars = SOME m
-Proof
-  ho_match_mp_tac toFloVerPre_ind
-  \\ rpt strip_tac \\ fs[toFloVerPre_def]
-  \\ qpat_x_assum ‘_ = SOME (_, _)’ mp_tac
-  \\ reverse TOP_CASE_TAC \\ fs[]
-  >- (
-    rpt (TOP_CASE_TAC \\ fs[])
-    \\ first_assum (mp_then Any assume_tac getInterval_inv)
-    \\ rpt strip_tac \\ fs[] \\ rveq
-    \\ first_assum (mp_then Any assume_tac lookupCMLVar_id_l)
-    \\ rveq \\ fsrw_tac [SATISFY_ss] [updateTheory.FIND_def])
-  \\ rpt (TOP_CASE_TAC \\ fs[])
-  \\ rpt strip_tac \\ rveq
-  \\ fs[freevars_def]
-  >- (
-    first_assum (mp_then Any assume_tac getInterval_inv)
-    \\ first_assum (mp_then Any assume_tac lookupCMLVar_id_l)
-    \\ fs[] \\ rveq
-    \\ fsrw_tac [SATISFY_ss] [updateTheory.FIND_def])
-  \\ res_tac
-  \\ imp_res_tac lookupCMLVar_id_l \\ rveq
-  \\ fsrw_tac [SATISFY_ss] [updateTheory.FIND_def]
-  \\ TOP_CASE_TAC \\ fs[]
-QED
-
-(* TODO: Move to HOL4 distrib *)
-Theorem float_is_finite_sandwich:
-  ∀ (w1:('a,'b) float) (w2:('a,'b) float) (w3:('a,'b) float).
-  float_less_equal w1 w2 ∧
-  float_less_equal w2 w3 ∧
-  float_is_finite w1 ∧
-  float_is_finite w3 ⇒
-  float_is_finite w2
-Proof
-  rpt strip_tac
-  \\ fs[binary_ieeeTheory.float_is_finite_def,
-        binary_ieeeTheory.float_less_equal_def]
-  \\ Cases_on ‘float_value w1’ \\ fs[]
-  \\ Cases_on ‘float_value w3’ \\ fs[]
-  \\ Cases_on ‘float_compare w1 w2’ \\ fs[]
-  \\ Cases_on ‘float_compare w2 w3’ \\ rfs[binary_ieeeTheory.float_compare_def]
-  \\ Cases_on ‘float_value w2’ \\ fs[]
-  \\ Cases_on ‘w2.Sign = 1w’ \\ fs[]
-QED
-
-Theorem fp64_isFinite_sandwich:
-  ∀ w1 w2 w3.
-    fp64_lessEqual w1 w2 ∧
-    fp64_lessEqual w2 w3 ∧
-    fp64_isFinite w1 ∧
-    fp64_isFinite w3 ⇒
-    fp64_isFinite w2
-Proof
-  fs[fp64_lessEqual_def, fp64_isFinite_def]
-  \\ rpt strip_tac
-  \\ irule float_is_finite_sandwich
-  \\ fsrw_tac [SATISFY_ss] []
-QED
+*)
 
 (**
   If toFloVerPre constructs a precondition from a CakeML precondition
@@ -230,70 +156,73 @@ Proof
   \\ imp_res_tac toFloVerPre_freevar_FIND \\ fs[] \\ rveq \\ fs[]
 QED
 
+(**
+  Relation: v_eq
+  Arguments:
+    The CakeML value v, a real number r, and a FloVer type m.
+  The predicate returns true, iff either m is REAL, and v represents exactly the
+  real number r, or m is M64 for a 64-bit double number, v is a double value or
+  a value tree, and r is the translation to reals of v. **)
 Definition v_eq_def:
-  v_eq (FP_WordTree fp) r = (r = fp64_to_real (compress_word fp)) ∧
-  v_eq (Litv (Word64 w)) r = (r = fp64_to_real w) ∧
-  v_eq _ _ = F
+  v_eq (FP_WordTree fp) r M64 = (r = fp64_to_real (compress_word fp)) ∧
+  v_eq (Litv (Word64 w)) r M64 = (r = fp64_to_real w) ∧
+  v_eq (Real r1) r2 REAL = (r1 = r2) ∧
+  v_eq _ _ _ = F
 End
+
+Triviality v_eq_float:
+  v_eq (Litv (Word64 w)) r m ⇔ ((m = M64) ∧ r = fp64_to_real w)
+Proof
+  Cases_on ‘m’ \\ fs[v_eq_def]
+QED
+
+Triviality v_eq_valtree:
+  v_eq (FP_WordTree fp) r m ⇔ ((m = M64) ∧ r = fp64_to_real (compress_word fp))
+Proof
+  Cases_on ‘m’ \\ fs[v_eq_def]
+QED
+
+Triviality v_eq_real:
+  v_eq v r REAL ⇔ v = Real r
+Proof
+  Cases_on ‘v’ \\ fs[v_eq_def]
+QED
 
 (**
   Relation: env_sim
   Arguments:
     The CakeML environment env, the FloVer environment E, and a set of pairs of
-    CakeML * FloVer variables
+    CakeML * FloVer variables, and a type environment Gamma
   The environments env and E are in relation with each other for the set of
-  variables fVars, if and only if the for every pair of variables
-  (cake_id, flover_id):
-  whenever the CakeML environment binds the the variable cake_id to a 64-bit
-  word, the FloVer environment binds flover_id to the words real equivalent, and
-  whenever the CakeM environment binds the variable to a value tree,
-  the FloVer environment binds flover_id to the real equivalent of the
-  compressed tree **)
+  variables fVars under the type assignment Gamma,
+  if and only if for every pair of variables (cake_id, flover_id):
+  if the CakeML environment binds cake_id, the FloVer environment must bind
+  flover_id to a value r that is in relation with the CakeML value for the type
+  in Gamma, and
+  if the FloVer environment binds flover_id, and has a type in Gamma, the
+  the CakeML environment binds the variable cake_id to a value that is in
+  relation with the FloVer value under the type from Gamma **)
 Definition env_sim_def:
-  env_sim env E fVars =
+  env_sim env E fVars Gamma =
     (∀ (cake_id:(string, string) id) (flover_id:num).
-      (cake_id, flover_id) IN fVars ⇒
-      (∀ v. ∃ r.
-      nsLookup env cake_id = SOME v ⇒
-      E flover_id = SOME r ∧ v_eq v r) ∧
-      (∀ r. ∃ v.
-      E flover_id = SOME r ⇒
-      nsLookup env cake_id = SOME v ∧ v_eq v r))
-End
-
-Definition ids_unique_def:
-  ids_unique ids =
-  ((∀ x y z.
-    lookupCMLVar x ids = SOME (x, y) ∧
-    lookupFloVerVar z ids = SOME (x, z) ⇒
-    z = y) ∧
-  (∀ x y z.
-    lookupCMLVar (Short x) ids = SOME (Short x, z) ∧
-    lookupFloVerVar z ids = SOME (Short y, z) ⇒
-    x = y) ∧
-  (∀ x y z.
-    lookupCMLVar x ids = SOME (x,z) ∧
-    lookupCMLVar y ids = SOME (y,z) ⇒
-    x = y) ∧
-  (∀ x y z.
-    lookupFloVerVar x ids = SOME (z,x) ∧
-    lookupFloVerVar y ids = SOME (z,y) ⇒
-    x = y) ∧
-  (∀ x y.
-    lookupFloVerVar x ids = SOME (y, x) ⇒
-    lookupCMLVar y ids = SOME (y,x)) ∧
-  (∀ x y.
-    lookupCMLVar y ids = SOME (y,x) ⇒
-    lookupFloVerVar x ids = SOME (y, x)))
+     (cake_id, flover_id) IN fVars ⇒
+      (∀ v.
+        nsLookup env cake_id = SOME v ⇒
+        ∃ r m. E flover_id = SOME r ∧ Gamma (Var flover_id) = SOME m ∧ v_eq v r m) ∧
+      (∀ r m.
+       E flover_id = SOME r ∧
+       Gamma (Var flover_id) = SOME m ⇒
+        ∃ v. nsLookup env cake_id = SOME v ∧ v_eq v r m))
 End
 
 Theorem getInterval_preserves_bounds:
-  ∀ e lo hi (st:α semanticPrimitives$state) env st2 E ids fVars x y z.
+  ∀ e lo hi (st:α semanticPrimitives$state) env st2 E ids
+    freshId fVars x y z (Gamma:real expr -> mType option).
     getInterval e = SOME (x, lo, hi) ∧
     st.fp_state.canOpt = FPScope NoOpt ∧
     evaluate st env [e] = (st2, Rval [Boolv T]) ∧
-    env_sim env.v E fVars ∧
-    ids_unique ids ∧
+    env_sim env.v E fVars Gamma ∧
+    ids_unique ids freshId ∧
     (∀ x. x IN freevars [e] ⇒ ∃ y. lookupCMLVar x ids = SOME (x,y) ∧ (x,y) IN fVars) ∧
     lookupFloVerVar y ids = SOME (Short x, y) ∧
     lookupCMLVar (Short x) ids = SOME (Short x, z) ⇒
@@ -308,41 +237,41 @@ Proof
   \\ ‘y = z’ by (fs[ids_unique_def])
   \\ rveq \\ fs[]
   \\ qpat_x_assum ‘evaluate _ _ _ = _’ mp_tac
-  \\ simp[terminationTheory.evaluate_def]
+  \\ simp[evaluate_def]
   \\ Cases_on ‘nsLookup env.v (Short x)’
-  \\ simp[astTheory.getOpClass_def, astTheory.isFpBool_def,
-          semanticPrimitivesTheory.do_app_def,
-          semanticPrimitivesTheory.fp_translate_def]
+  \\ simp[astTheory.getOpClass_def, astTheory.isFpBool_def, do_app_def,
+          fp_translate_def]
   \\ rename1 ‘nsLookup env.v (Short x) = SOME v’
   \\ fs[env_sim_def] \\ first_x_assum (qspecl_then [‘Short x’, ‘y’] assume_tac)
   \\ rfs[]
-  \\ Cases_on ‘v’ \\ simp[semanticPrimitivesTheory.fp_translate_def]
+  \\ Cases_on ‘v’ \\ simp[fp_translate_def]
   THENL [rename1 ‘Litv l’ \\ Cases_on ‘l’
-         \\ simp [semanticPrimitivesTheory.fp_translate_def],
+         \\ simp [fp_translate_def],
          ALL_TAC]
-  \\ simp [semanticPrimitivesTheory.do_log_def,
-           fpValTreeTheory.fp_cmp_def, fpSemTheory.fp_cmp_comp_def,
+  \\ simp [do_log_def, fpValTreeTheory.fp_cmp_def, fpSemTheory.fp_cmp_comp_def,
            fpSemTheory.compress_word_def, fpSemTheory.compress_bool_def]
   THENL [
     Cases_on ‘fp64_lessEqual w1 c’,
     Cases_on ‘fp64_lessEqual w1 (compress_word f)’]
-  \\ simp[terminationTheory.evaluate_def, astTheory.getOpClass_def,
-          astTheory.isFpBool_def, semanticPrimitivesTheory.do_app_def,
-          semanticPrimitivesTheory.fp_translate_def]
+  \\ simp[evaluate_def, astTheory.getOpClass_def,
+          astTheory.isFpBool_def, do_app_def, fp_translate_def]
   \\ simp[fpValTreeTheory.fp_cmp_def, fpSemTheory.fp_cmp_comp_def,
           fpSemTheory.compress_word_def, fpSemTheory.compress_bool_def]
   \\ rpt strip_tac \\ rveq
-  THENL [
-     first_x_assum (qspec_then ‘Litv (Word64 c)’ assume_tac),
-     first_x_assum (qspec_then ‘FP_WordTree f’ assume_tac)]
-  \\ fs[v_eq_def]
-  \\ fs[fp64_to_real_def, fp64_isFinite_def, fp64_lessEqual_def]
+  \\ first_x_assum (qspec_then ‘r’ assume_tac)
+  \\ fs[v_eq_def, fp64_to_real_def, fp64_isFinite_def, fp64_lessEqual_def]
   THENL [
     ‘float_is_finite (fp64_to_float c)’
       by (irule float_is_finite_sandwich \\ fsrw_tac [SATISFY_ss] []),
+    ‘float_is_finite (fp64_to_float c)’
+      by (irule float_is_finite_sandwich \\ fsrw_tac [SATISFY_ss] []),
+    ‘float_is_finite (fp64_to_float (compress_word f))’
+      by (irule float_is_finite_sandwich \\ fsrw_tac [SATISFY_ss] []),
     ‘float_is_finite (fp64_to_float (compress_word f))’
       by (irule float_is_finite_sandwich \\ fsrw_tac [SATISFY_ss] [])]
-  \\ conj_tac \\ metis_tac [lift_ieeeTheory.float_le]
+  \\ res_tac
+  \\ fs[v_eq_float, v_eq_valtree] \\ rveq \\ simp[fp64_to_real_def]
+  \\ metis_tac [lift_ieeeTheory.float_le]
 QED
 
 (**
@@ -353,14 +282,14 @@ QED
   of the precondition, then the FloVer environment must respect the precondition
   too **)
 Theorem toFloVerPre_preserves_bounds:
-  ∀ cake_P ids floverP dVars.
+  ∀ cake_P ids floverP dVars (Gamma:real expr -> mType option).
     (* We can extract a precondition *)
     toFloVerPre cake_P (ids:((string, string) id # num) list) = SOME (floverP,dVars) ⇒
-    ∀ st (st2:α semanticPrimitives$state) env E fVars.
+    ∀ st (st2:α semanticPrimitives$state) env E fVars freshId.
       st.fp_state.canOpt = FPScope NoOpt ∧
       (* the free variables are paired up in the id list, and defined *)
-      env_sim env.v E fVars ∧
-      ids_unique ids ∧
+      env_sim env.v E fVars Gamma ∧
+      ids_unique ids freshId ∧
       (∀ x. x IN freevars cake_P ⇒ ∃ y. lookupCMLVar x ids = SOME (x,y) ∧ (x,y) IN fVars) ∧
       (* the precondition can be evaluated to True *)
       evaluate st env cake_P = (st2, Rval ([Boolv T])) ⇒
@@ -387,14 +316,14 @@ Proof
   \\ rpt (TOP_CASE_TAC \\ fs[])
   \\ rpt strip_tac \\ rveq
   \\ qpat_x_assum ‘evaluate _ _ _ = _’ mp_tac
-  \\ simp[terminationTheory.evaluate_def]
+  \\ simp[evaluate_def]
   \\ ntac 2 (TOP_CASE_TAC \\ fs[])
-  \\ simp[semanticPrimitivesTheory.do_log_def]
+  \\ simp[do_log_def]
   \\ rename1 ‘evaluate st env [e1] = (st1, Rval v)’
   \\ reverse (Cases_on ‘HD v = Boolv T’) \\ fs[]
   >- (Cases_on ‘HD v = Boolv F’ \\ fs[])
   \\ strip_tac \\ fs[]
-  \\ first_x_assum (qspecl_then [‘st1’, ‘st2’, ‘env’, ‘E’, ‘fVars’] mp_tac)
+  \\ first_x_assum (qspecl_then [‘Gamma’,‘st1’, ‘st2’, ‘env’, ‘E’, ‘fVars’, ‘freshId’] mp_tac)
   \\ impl_tac \\ fs[]
   >- (imp_res_tac fpSemPropsTheory.evaluate_fp_opts_inv \\ fs[freevars_def])
   \\ rpt strip_tac \\ imp_res_tac evaluatePropsTheory.evaluate_sing
@@ -424,87 +353,462 @@ Proof
   \\ simp[toFloVerPre_def] \\ rveq \\ fs[]
 QED
 
-Theorem prepareVars_is_unique:
-  ∀ ids floverVars varMap freshId.
-    prepareVars ids = (floverVars, varMap, freshId) ⇒
-    ids_unique varMap ∧
-    (∀ id. freshId ≤ id ⇒ lookupFloVerVar id varMap = NONE) ∧
-    (∀ x y. lookupCMLVar x varMap = SOME (x, y) ⇒
-     y < freshId)
+Theorem approxEnv_construct:
+  ∀ E1 Gamma A fVars.
+    (∀ x. ~ (x  IN domain fVars) ⇒ E1 x = NONE) ∧
+    (∀ x. x IN domain fVars ⇒ Gamma (Var x) = SOME M64) ∧
+    (∀ x. x IN domain fVars ⇒ ∃ v. E1 x = SOME v) ∧
+    (∀ x v. E1 x = SOME v ⇒ (normalizes (:52 # 11) v ∨ v = 0)) ⇒
+    approxEnv E1
+              Gamma A fVars LN
+              (toREnv
+               (λ n. case E1 n of
+                |NONE => NONE
+                | SOME v => SOME (float_to_fp64 (round roundTiesToEven v))))
 Proof
-  Induct_on ‘ids’ \\ fs[prepareVars_def]
+  fs[approxEnv_def] \\ rpt strip_tac
   >- (
-    rpt strip_tac \\ fs[] \\ rveq
-    \\ fs[ids_unique_def, lookupCMLVar_def, lookupFloVerVar_def,
-          updateTheory.FIND_def])
-  \\ Cases_on ‘prepareVars ids’ \\ rename1 ‘prepareVars ids = (floverVars, p)’
-  \\ Cases_on ‘p’ \\ rename1 ‘prepareVars ids = (floverVars, varMap, freshId)’
-  \\ fs[ids_unique_def] \\ rpt strip_tac \\ rpt conj_tac
-  \\ fs[appendCMLVar_def]
-  \\ Cases_on ‘lookupCMLVar (Short h) varMap’
-  \\ fs[lookupCMLVar_def, lookupFloVerVar_def, updateTheory.FIND_def]
-  \\ every_case_tac \\ rveq \\ fs[]
-  \\ res_tac \\ rveq \\ fs[]
+    res_tac \\ fs[toREnv_def])
+  \\ res_tac \\ fs[toREnv_def]
+  \\ simp[fp64_to_float_float_to_fp64]
+  \\ ‘normalizes (:52 # 11) v ∨ v = 0’
+    by (first_x_assum irule \\ fsrw_tac [SATISFY_ss] [])
+  >- (
+    imp_res_tac lift_ieeeTheory.relative_error
+    \\ simp[MachineTypeTheory.computeError_def, MachineTypeTheory.mTypeToR_def]
+    \\ rewrite_tac [REAL_LDISTRIB, REAL_MUL_RID, real_sub, REAL_NEG_ADD,
+                    REAL_ADD_ASSOC]
+    \\ fs[ABS_NEG, ABS_MUL]
+    \\ irule REAL_LE_RMUL_IMP \\ fs[ABS_POS])
+  \\ rveq \\ fs[binary_ieeeTheory.round_def, binary_ieeeTheory.threshold]
+  \\ Q.ISPEC_THEN ‘f:(52,11) float’
+                  (assume_tac o SIMP_RULE std_ss [] o GEN_ALL) closest_such_0
+  \\ fs[binary_ieeeTheory.zero_to_real, MachineTypeTheory.computeError_def]
 QED
 
-Theorem toFloVerExp_noDowncast:
-  ∀ varMap freshId e theIds freshId2 theExp.
-    toFloVerExp varMap freshId e = SOME (theIds, freshId2, theExp) ⇒
-    noDowncast (toRExp theExp)
-Proof
-  ho_match_mp_tac toFloVerExp_ind
-  \\ rpt strip_tac \\ fs[toFloVerExp_def, toRExp_def, noDowncast_def]
-  \\ rveq \\ fs[toRExp_def, noDowncast_def]
-  \\ every_case_tac \\ fs[] \\ rveq
-  \\ fs[toRExp_def, noDowncast_def]
-QED
-
-Theorem toFloVerCmd_noDowncastFun:
-  ∀ varMap freshId f theIds freshId2 theCmd.
-    toFloVerCmd varMap freshId f = SOME (theIds, freshId2, theCmd) ⇒
-    noDowncastFun (toRCmd theCmd)
-Proof
-  ho_match_mp_tac toFloVerCmd_ind
-  \\ rpt strip_tac \\ fs[toFloVerCmd_def, toRCmd_def, noDowncastFun_def]
-  \\ every_case_tac \\ fs[toRCmd_def, noDowncastFun_def] \\ rveq
-  \\ fs[toRCmd_def, noDowncastFun_def]
-  \\ irule toFloVerExp_noDowncast \\ asm_exists_tac \\ fs[]
-QED
-
-Theorem is64BitEnv_prepareGamma:
+Theorem prepareGamma_is_64Bit:
   ∀ floverVars. is64BitEnv (prepareGamma floverVars)
 Proof
-  Induct_on ‘floverVars’ \\ fs[is64BitEnv_def, prepareGamma_def]
-  >- (
-   rpt strip_tac
-   \\ fs[FloverMapTheory.FloverMapTree_find_def,
-         FloverMapTheory.FloverMapTree_empty_def])
-  \\ rpt strip_tac \\ fs[FloverMapTheory.map_find_add]
-  \\ every_case_tac \\ fs[] \\ res_tac
+  Induct_on ‘floverVars’
+  \\ fs[prepareGamma_def, is64BitEnv_def,
+        FloverMapTree_empty_def, FloverMapTree_find_def, map_find_add]
+  \\ rpt strip_tac \\ every_case_tac \\ rveq
+  \\ fs[ExpressionAbbrevsTheory.toRExpMap_def, FloverMapTheory.map_find_add]
+  \\ res_tac
 QED
 
-Theorem toFloVerExp_is64BitEval:
-  ∀ varMap freshId e theIds freshId2 theExp.
-    toFloVerExp varMap freshId e = SOME (theIds, freshId2, theExp) ⇒
-    is64BitEval (toRExp theExp)
+Theorem eval_expr_real:
+  ∀ Gamma E e v m.
+  (∀ x m. Gamma x = SOME m ⇒ m = REAL) ∧
+  eval_expr E Gamma (toREval e) v m ⇒
+  m = REAL
+Proof
+  Induct_on ‘e’ \\ rpt strip_tac
+  \\ fs[Once toREval_def, Once eval_expr_cases] \\ rveq
+  \\ res_tac
+QED
+
+Theorem CakeML_FloVer_real_sim_exp:
+  ∀ varMap freshId f theIds freshId2 theExp E env fVars st Gamma v.
+    toFloVerExp varMap freshId f = SOME (theIds, freshId2, theExp) ∧
+    ids_unique varMap freshId ∧
+    st.fp_state.real_sem ∧
+    env_sim env.v E fVars Gamma ∧
+    (∀ x m. Gamma x = SOME m ⇒ m = REAL) ∧
+    (∀ x. x IN freevars [f] ⇒ ∃ y. lookupCMLVar x varMap = SOME (x,y) ∧ (x,y) IN fVars) ∧
+    eval_expr E Gamma (toREval (toRExp theExp)) v REAL ⇒
+    ∃ st2. evaluate st env [toRealExp f] = (st2, Rval [Real v])
 Proof
   ho_match_mp_tac toFloVerExp_ind
-  \\ rpt strip_tac \\ fs[toFloVerExp_def, toRExp_def, is64BitEval_def]
-  \\ rveq \\ fs[toRExp_def, is64BitEval_def]
-  \\ every_case_tac \\ fs[] \\ rveq
-  \\ fs[toRExp_def, is64BitEval_def]
+  \\ rpt strip_tac
+  \\ ((rename1 ‘App op exps’ \\ imp_res_tac toFloVerExp_App_cases)
+     ORELSE
+     (qpat_x_assum ‘toFloVerExp _ _ _ = SOME _’ mp_tac
+      \\ simp[Once toFloVerExp_def] \\ rpt strip_tac))
+  \\ rveq \\ fs[toRealExp_def, freevars_def]
+  \\ rfs[] \\ rveq \\ fs [toRExp_def, toREval_def, eval_expr_cases]
+  >- (
+    fs[env_sim_def] \\ rveq \\ fs[ExpressionAbbrevsTheory.toRExpMap_def]
+    \\ simp[evaluate_def] \\ res_tac \\ fs[v_eq_real])
+  >- (
+    simp[toRealExp_def, evaluate_def, astTheory.getOpClass_def]
+    \\ fs[MachineTypeTheory.mTypeToR_def, perturb_def] \\ rveq
+    \\ simp[do_app_def, fp64_to_real_def])
+  >- (
+    rveq \\ rpt (qpat_x_assum ‘T’ kall_tac)
+    \\ fs[freevars_def]
+    \\ ‘∃ st2. evaluate st env [toRealExp e] = (st2, Rval [Real v1])’
+      by (
+        last_x_assum drule \\ rpt (disch_then drule)
+        \\ Cases_on ‘m'’ \\ fs[MachineTypeTheory.isCompat_def])
+    \\ simp[toRealExp_def, evaluate_def, astTheory.getOpClass_def,
+            getRealUop_def]
+    \\ ‘st2.fp_state.real_sem’
+      by (imp_res_tac fpSemPropsTheory.evaluate_fp_opts_inv)
+    \\ fs[do_app_def]
+    \\ EVAL_TAC \\ fs[])
+  >- (
+    imp_res_tac toFloVerExp_ids_unique
+    \\ rveq \\ rpt (qpat_x_assum ‘T’ kall_tac)
+    \\ fs[freevars_def]
+    \\ ‘m1 = REAL ∧ m2 = REAL’
+       by (
+         conj_tac \\ irule eval_expr_real
+         \\ once_rewrite_tac[CONJ_COMM] \\ asm_exists_tac \\ fs[]
+         \\ first_x_assum MATCH_ACCEPT_TAC)
+    \\ rveq
+    \\ ‘∃ st2. evaluate st env [toRealExp e2] = (st2, Rval [Real v2])’
+      by (
+        last_x_assum drule \\ rpt (disch_then drule)
+        \\ disch_then (qspec_then ‘v2’ mp_tac) \\ impl_tac \\ fs[]
+        \\ rpt strip_tac
+        \\ first_x_assum (qspec_then ‘x’ mp_tac) \\ fs[]
+        \\ imp_res_tac toFloVerExp_lookup_mono
+        \\ strip_tac \\ fs[]
+        \\ res_tac
+        \\ fsrw_tac [SATISFY_ss] [])
+    \\ ‘st2.fp_state.real_sem’
+      by (imp_res_tac fpSemPropsTheory.evaluate_fp_opts_inv)
+    \\ ‘∃ st3. evaluate st2 env [toRealExp e1] = (st3, Rval [Real v1])’
+      by (
+        last_x_assum kall_tac
+        \\ last_x_assum drule \\ rpt (disch_then drule)
+        \\ disch_then (qspec_then ‘v1’ mp_tac) \\ impl_tac \\ fs[]
+        \\ rpt strip_tac
+        \\ first_x_assum (qspec_then ‘x’ mp_tac) \\ fs[])
+    \\ ‘st3.fp_state.real_sem’
+      by (imp_res_tac fpSemPropsTheory.evaluate_fp_opts_inv)
+    \\ simp[evaluate_def, astTheory.getOpClass_def, semanticPrimitivesTheory.do_app_def]
+    \\ fs[MachineTypeTheory.mTypeToR_def, perturb_def]
+    \\ Cases_on ‘bop’ \\ EVAL_TAC)
+  >- (
+    imp_res_tac toFloVerExp_ids_unique
+    \\ rveq \\ rpt (qpat_x_assum ‘T’ kall_tac)
+    \\ fs[freevars_def]
+    \\ ‘m1 = REAL ∧ m2 = REAL ∧ m3 = REAL’
+       by (
+         rpt conj_tac \\ irule eval_expr_real
+         \\ once_rewrite_tac[CONJ_COMM] \\ asm_exists_tac \\ fs[]
+         \\ first_x_assum MATCH_ACCEPT_TAC)
+    \\ rveq
+    \\ ‘∀ st. st.fp_state.real_sem ⇒ ∃ st2. evaluate st env [toRealExp e3] = (st2, Rval [Real v3])’
+      by (
+        rpt strip_tac
+        \\ last_x_assum drule \\ rpt (disch_then drule)
+        \\ disch_then (qspec_then ‘v3’ mp_tac)
+        \\ impl_tac \\ fs[]
+        \\ rpt strip_tac
+        \\ first_x_assum (qspec_then ‘x’ mp_tac) \\ fs[]
+        \\ strip_tac
+        \\ imp_res_tac toFloVerExp_lookup_mono
+        \\ res_tac
+        \\ fsrw_tac [SATISFY_ss] [])
+    \\ last_x_assum kall_tac
+    \\ ‘∀ st. st.fp_state.real_sem ⇒ ∃ st2. evaluate st env [toRealExp e2] = (st2, Rval [Real v2])’
+      by (
+        rpt strip_tac
+        \\ last_x_assum drule \\ rpt (disch_then drule)
+        \\ disch_then (qspec_then ‘v2’ mp_tac) \\ impl_tac \\ fs[]
+        \\ rpt strip_tac
+        \\ first_x_assum (qspec_then ‘x’ mp_tac) \\ fs[]
+        \\ imp_res_tac toFloVerExp_lookup_mono
+        \\ strip_tac \\ fs[]
+        \\ res_tac
+        \\ fsrw_tac [SATISFY_ss] [])
+    \\ last_x_assum kall_tac
+    \\ ‘∀ st. st.fp_state.real_sem ⇒ ∃ st2. evaluate st env [toRealExp e1] = (st2, Rval [Real v1])’
+      by (
+        rpt strip_tac
+        \\ last_x_assum drule \\ rpt (disch_then drule)
+        \\ disch_then (qspec_then ‘v1’ mp_tac) \\ impl_tac \\ fs[]
+        \\ rpt strip_tac
+        \\ first_x_assum (qspec_then ‘x’ mp_tac) \\ fs[]
+        \\ imp_res_tac toFloVerExp_lookup_mono
+        \\ strip_tac \\ fs[]
+        \\ res_tac
+        \\ fsrw_tac [SATISFY_ss] [])
+    \\ last_x_assum kall_tac
+    \\ first_x_assum (qspec_then ‘st’ mp_tac) \\ impl_tac \\ fs[]
+    \\ strip_tac \\ fs[]
+    \\ ‘st2.fp_state.real_sem’
+      by (imp_res_tac fpSemPropsTheory.evaluate_fp_opts_inv)
+    \\ last_x_assum (qspec_then ‘st2’ mp_tac) \\ impl_tac \\ fs[]
+    \\ strip_tac \\ fs[]
+    \\ rename1 ‘evaluate st2 env [toRealExp e3] = (st3, Rval [Real v3])’
+    \\ ‘st3.fp_state.real_sem’
+      by (imp_res_tac fpSemPropsTheory.evaluate_fp_opts_inv)
+    \\ last_x_assum (qspec_then ‘st3’ mp_tac) \\ impl_tac \\ fs[]
+    \\ strip_tac \\ fs[]
+    \\ rename1 ‘evaluate st3 env [toRealExp e2] = (st4, Rval [Real v2])’
+    \\ ‘st4.fp_state.real_sem’
+      by (imp_res_tac fpSemPropsTheory.evaluate_fp_opts_inv)
+    \\ simp[evaluate_def, astTheory.getOpClass_def,
+            semanticPrimitivesTheory.do_app_def]
+    \\ simp[evaluateTheory.shift_fp_opts_def]
+    \\ fs[MachineTypeTheory.mTypeToR_def, perturb_def]
+    \\ EVAL_TAC \\ REAL_ARITH_TAC)
 QED
 
-Theorem toFloVerCmd_is64BitBstep:
-  ∀ varMap freshId f theIds freshId2 theCmd.
-    toFloVerCmd varMap freshId f = SOME (theIds, freshId2, theCmd) ⇒
-    is64BitBstep (toRCmd theCmd)
+Theorem CakeML_FloVer_real_sim:
+  ∀ varMap freshId f theIds freshId2 theCmd E env fVars st Gamma r.
+    toFloVerCmd varMap freshId f = SOME (theIds, freshId2, theCmd) ∧
+    ids_unique varMap freshId ∧
+    st.fp_state.real_sem ∧
+    env_sim env.v E fVars Gamma ∧
+    (∀ x m. Gamma x = SOME m ⇒ m = REAL) ∧
+    (∀ x y. (x,y) IN fVars ⇒ lookupCMLVar x varMap = SOME (x,y)) ∧
+    (∀ x. x IN freevars [f] ⇒ ∃ y. lookupCMLVar x varMap = SOME (x,y) ∧ (x,y) IN fVars) ∧
+    bstep (toREvalCmd (toRCmd theCmd)) E Gamma r REAL ⇒
+    ∃ st2. evaluate st env [toRealExp f] = (st2, Rval [Real r])
 Proof
   ho_match_mp_tac toFloVerCmd_ind
-  \\ rpt strip_tac \\ fs[toFloVerCmd_def, toRCmd_def, is64BitBstep_def]
-  \\ every_case_tac \\ fs[toRCmd_def, is64BitBstep_def] \\ rveq
-  \\ fs[toRCmd_def, is64BitBstep_def]
-  \\ irule toFloVerExp_is64BitEval \\ asm_exists_tac \\ fs[]
+  \\ rpt strip_tac \\ fs[toFloVerCmd_def]
+  >- (
+   fs[option_case_eq, pair_case_eq] \\ rveq
+   \\ qpat_x_assum ‘bstep _ _ _ _ _’ mp_tac
+   \\ simp[Once toRCmd_def, Once toREvalCmd_def, bstep_cases, freevars_def]
+   \\ rpt strip_tac
+   \\ drule CakeML_FloVer_real_sim_exp \\ rpt (disch_then drule)
+   \\ disch_then (qspec_then ‘v’ mp_tac) \\ impl_tac \\ fs[freevars_def]
+   \\ disch_then assume_tac \\ fs[]
+   \\ ‘st2.fp_state.real_sem’
+      by (imp_res_tac fpSemPropsTheory.evaluate_fp_opts_inv)
+   \\ qpat_assum ‘bstep _ _ _ _ _’
+                   (fn thm => first_x_assum (fn ithm => mp_then Any mp_tac ithm thm))
+   \\ disch_then
+      (qspecl_then [‘env with v := (nsOptBind (SOME x) (Real v) env.v)’,
+                    ‘fVars UNION { (Short x,freshId2')}’,
+                    ‘st2’] mp_tac)
+   \\ impl_tac
+   >- (
+     rpt conj_tac \\ fs[]
+     >- (
+       irule ids_unique_append
+       \\ irule toFloVerExp_ids_unique \\ asm_exists_tac \\ fs[])
+     >- (
+       simp[env_sim_def] \\ rpt strip_tac \\ fs[namespaceTheory.nsOptBind_def]
+       >- (
+         ‘cake_id ≠ Short x’
+          by (CCONTR_TAC
+              \\ fs[] \\ rveq \\ res_tac
+              \\ imp_res_tac toFloVerExp_lookup_mono \\ fs[])
+         \\ ‘flover_id ≠ freshId2'’
+           by (CCONTR_TAC
+               \\ fs[] \\ rveq \\ res_tac
+               \\ imp_res_tac toFloVerExp_ids_unique
+               \\ imp_res_tac toFloVerExp_lookup_mono
+               \\ fs[ids_unique_def] \\ res_tac
+               \\ fs[])
+         \\ fs[env_sim_def] \\ res_tac
+         \\ fsrw_tac [SATISFY_ss] []
+         \\ res_tac \\ fs[])
+       >- (
+         ‘cake_id ≠ Short x’
+          by (CCONTR_TAC
+              \\ fs[] \\ rveq \\ res_tac
+              \\ imp_res_tac toFloVerExp_lookup_mono \\ fs[])
+         \\ ‘flover_id ≠ freshId2'’
+           by (CCONTR_TAC
+               \\ fs[] \\ rveq \\ res_tac
+               \\ imp_res_tac toFloVerExp_ids_unique
+               \\ imp_res_tac toFloVerExp_lookup_mono
+               \\ fs[ids_unique_def] \\ res_tac
+               \\ fs[])
+         \\ fs[ml_progTheory.nsLookup_nsBind_compute]
+         \\ fs[env_sim_def] \\ res_tac
+         \\ fsrw_tac [SATISFY_ss] []
+         \\ res_tac \\ rfs[])
+       >- (
+         rveq \\ fs[ml_progTheory.nsLookup_nsBind_compute]
+         \\ rveq \\ fs[v_eq_def])
+       \\ rveq \\ fs[] \\ rveq \\ fs[v_eq_def])
+     >- (
+      rpt strip_tac
+      >- (
+        fs[lookupCMLVar_appendCMLVar]
+        \\ ‘x' ≠ Short x’
+          by (CCONTR_TAC
+              \\ fs[] \\ rveq \\ res_tac
+              \\ imp_res_tac toFloVerExp_lookup_mono \\ fs[])
+         \\ ‘y ≠ freshId2'’
+           by (CCONTR_TAC
+               \\ fs[] \\ rveq \\ res_tac
+               \\ imp_res_tac toFloVerExp_ids_unique
+               \\ imp_res_tac toFloVerExp_lookup_mono
+               \\ fs[ids_unique_def] \\ res_tac
+               \\ fs[])
+         \\ res_tac
+         \\ imp_res_tac toFloVerExp_lookup_mono
+         \\ fs[lookupCMLVar_def, updateTheory.FIND_def])
+      \\ rveq \\ fs[lookupCMLVar_appendCMLVar, lookupCMLVar_def, updateTheory.FIND_def])
+     >- (
+       rpt strip_tac
+       \\ fs[lookupCMLVar_appendCMLVar, lookupCMLVar_def, updateTheory.FIND_def]
+       \\ TOP_CASE_TAC \\ fs[]
+       \\ first_x_assum (qspec_then ‘x'’ mp_tac) \\ fs[]
+       \\ disch_then assume_tac \\ fs[]
+       \\ imp_res_tac (SIMP_RULE std_ss [lookupCMLVar_def] toFloVerExp_lookup_mono)
+       \\ fs[]))
+    \\ disch_then assume_tac \\ fs[]
+    \\ simp[toRealExp_def, evaluate_def])
+  \\ fs[option_case_eq, pair_case_eq] \\ rveq
+  \\ fs[Once toRCmd_def, Once toREvalCmd_def, bstep_cases] \\ rveq
+  \\ drule CakeML_FloVer_real_sim_exp \\ fs[]
+  \\ rpt (disch_then drule) \\ fs[]
+QED
+
+Theorem CakeML_FloVer_float_sim_exp:
+  ∀ varMap freshId f theIds freshId2 theExp E env fVars st vF Gamma.
+    toFloVerExp varMap freshId f = SOME (theIds, freshId2, theExp) ∧
+    st.fp_state.canOpt = FPScope NoOpt ∧
+    ids_unique varMap freshId ∧
+    (∀ x m. (toRExpMap Gamma) x = SOME m ⇒ m = M64) ∧
+    (∀ x y. (x,y) IN fVars ⇒ lookupCMLVar x varMap = SOME (x,y)) ∧
+    env_sim env.v E fVars (toRExpMap Gamma) ∧
+    (∀ x. x IN freevars [f] ⇒ ∃ y. lookupCMLVar x varMap = SOME (x,y) ∧ (x,y) IN fVars) ∧
+    validTypes (toRExp theExp) Gamma ∧
+    eval_expr_float theExp
+      (λ x. case E x of NONE => NONE | SOME v => SOME (float_to_fp64 (round roundTiesToEven v))) =
+      SOME vF ⇒
+    ∃ vFC st2. evaluate st env [f] = (st2, Rval [vFC]) ∧ v_eq vFC (fp64_to_real vF) M64
+Proof
+  ho_match_mp_tac toFloVerExp_ind
+  \\ rpt strip_tac
+  \\ ((rename1 ‘App op exps’ \\ imp_res_tac toFloVerExp_App_cases)
+     ORELSE
+     (qpat_x_assum ‘toFloVerExp _ _ _ = SOME _’ mp_tac
+      \\ simp[Once toFloVerExp_def] \\ rpt strip_tac))
+  >- (
+    fs[option_case_eq, pair_case_eq] \\ rveq
+    \\ fs[eval_expr_float_def, option_case_eq, Once validTypes_def, toRExp_def,
+          ExpressionAbbrevsTheory.toRExpMap_def, freevars_def]
+    \\ rveq \\ fs[env_sim_def]
+    \\ res_tac \\ rveq \\ fs[] \\ rveq
+    \\ simp[evaluate_def]
+    \\ Cases_on ‘v'’ \\ fs[v_eq_def] \\ rveq
+    >- (
+      Cases_on ‘l’ \\ fs[v_eq_def] \\ rveq
+      \\ simp[fp64_to_real_def]
+      \\ ‘float_is_finite (fp64_to_float c) ∧ ~ float_is_zero (fp64_to_float c)’
+        by (cheat)
+      \\ fs[lift_ieeeTheory.round_finite_normal_float_id,
+            float_to_fp64_fp64_to_float])
+    >- (
+      ‘float_is_finite (fp64_to_float (compress_word f)) ∧
+          ~ float_is_zero (fp64_to_float (compress_word f))’
+        by (cheat)
+      \\ simp[fp64_to_real_def]
+      \\ fs[lift_ieeeTheory.round_finite_normal_float_id,
+            float_to_fp64_fp64_to_float]))
+  >- (
+    fs[option_case_eq, pair_case_eq] \\ rveq
+    \\ fs[eval_expr_float_def, option_case_eq, Once validTypes_def, toRExp_def,
+          ExpressionAbbrevsTheory.toRExpMap_def, freevars_def]
+    \\ rveq \\ fs[]
+    \\ simp[evaluate_def, v_eq_def])
+  >- (
+    fs[option_case_eq, pair_case_eq] \\ rveq
+    \\ rpt (qpat_x_assum ‘T’ kall_tac)
+    \\ fs[eval_expr_float_def, option_case_eq, toRExp_def,
+          ExpressionAbbrevsTheory.toRExpMap_def, freevars_def]
+    \\ rveq \\ fs[]
+    \\ ‘validTypes (toRExp fexp2) Gamma’
+       by (fs[Once validTypes_def])
+    \\ ‘∃ vFC st2. evaluate st env [e] = (st2, Rval [vFC]) ∧
+        v_eq vFC (fp64_to_real v) M64’
+      by (
+        last_x_assum drule \\ rpt (disch_then drule)
+        \\ disch_then assume_tac \\ fs[])
+    \\ ‘st2.fp_state.canOpt = FPScope NoOpt’
+       by (imp_res_tac fpSemPropsTheory.evaluate_fp_opts_inv \\ fs[])
+    \\ simp[evaluate_def, v_eq_def, astTheory.getOpClass_def, semanticPrimitivesTheory.do_app_def]
+    \\ Cases_on ‘vFC’ \\ fs[v_eq_def]
+    THENL [Cases_on ‘l’, ALL_TAC]
+    \\ fs[v_eq_def, semanticPrimitivesTheory.fp_translate_def,
+          astTheory.isFpBool_def, fpValTreeTheory.fp_uop_def,
+          fpSemTheory.compress_word_def]
+    >- (
+      EVAL_TAC
+      \\ fs[fp64_to_real_def, fp64_negate_def, fp64_to_float_float_to_fp64,
+            binary_ieeeTheory.float_to_real_negate])
+    \\ fs[fp64_to_real_def, binary_ieeeTheory.float_to_real_eq]
+    >- (
+      EVAL_TAC
+      \\ fs[fp64_negate_def, fp64_to_float_float_to_fp64])
+    \\ EVAL_TAC
+    \\ fs[fp64_negate_def, fp64_to_float_float_to_fp64, binary_ieeeTheory.float_to_real_negate]
+    \\ fs[binary_ieeeTheory.float_negate_def, binary_ieeeTheory.float_is_zero])
+  >- (
+    rveq \\ fs[]
+    \\ rpt (qpat_x_assum ‘T’ kall_tac)
+    \\ fs[eval_expr_float_def, option_case_eq, toRExp_def,
+          ExpressionAbbrevsTheory.toRExpMap_def, freevars_def]
+    \\ rveq \\ fs[]
+    \\ ‘validTypes (toRExp fexp1) Gamma’
+       by (fs[Once validTypes_def])
+    \\ ‘validTypes (toRExp fexp2) Gamma’
+       by (fs[Once validTypes_def])
+    \\ ‘∀ x y. (x,y) IN fVars ⇒ lookupCMLVar x theIds2 = SOME (x,y)’
+       by (rpt strip_tac \\ res_tac \\ imp_res_tac toFloVerExp_lookup_mono)
+    \\ ‘∃ vFC st2. evaluate st env [e2] = (st2, Rval [vFC]) ∧
+        v_eq vFC (fp64_to_real v2) M64’
+      by (
+        imp_res_tac toFloVerExp_ids_unique
+        \\ last_x_assum drule \\ rpt (disch_then drule)
+        \\ disch_then (qspec_then ‘v2’ mp_tac) \\ impl_tac \\ fs[]
+        >- (
+          rpt strip_tac \\ ntac 2 (first_x_assum (qspec_then ‘x’ mp_tac)) \\ fs[]
+          \\ rpt strip_tac
+          \\ imp_res_tac toFloVerExp_lookup_mono \\ fs[])
+        \\ disch_then assume_tac \\ fs[])
+    \\ ‘st2.fp_state.canOpt = FPScope NoOpt’
+      by (imp_res_tac fpSemPropsTheory.evaluate_fp_opts_inv \\ fs[])
+    \\ last_x_assum kall_tac
+    \\ ‘∃ vFC st3. evaluate st2 env [e1] = (st3, Rval [vFC]) ∧
+        v_eq vFC (fp64_to_real v1) M64’
+      by (
+        imp_res_tac toFloVerExp_ids_unique
+        \\ last_x_assum drule \\ rpt (disch_then drule)
+        \\ disch_then (qspec_then ‘v1’ mp_tac) \\ impl_tac \\ fs[])
+    \\ ‘st3.fp_state.canOpt = FPScope NoOpt’
+      by (imp_res_tac fpSemPropsTheory.evaluate_fp_opts_inv \\ fs[])
+    \\ simp[evaluate_def, v_eq_def, astTheory.getOpClass_def,
+            semanticPrimitivesTheory.do_app_def]
+    \\ Cases_on ‘vFC'’ \\ Cases_on ‘vFC’
+    \\ TRY (rename1 ‘v_eq (Litv l1) (fp64_to_real v1) M64’ \\ Cases_on ‘l1’)
+    \\ TRY (rename1 ‘v_eq (Litv l2) (fp64_to_real v2) M64’ \\ Cases_on ‘l2’)
+    \\ fs[v_eq_def, semanticPrimitivesTheory.fp_translate_def,
+          astTheory.isFpBool_def, fpValTreeTheory.fp_uop_def,
+          fpSemTheory.compress_word_def]
+     (* MARKER *)
+    \\ fs[fp64_to_real_def, binary_ieeeTheory.float_to_real_eq]
+    \\ Cases_on ‘bop’ \\ fs[fpBopToFloVer_def] \\ rveq
+    \\ fs[fpSemTheory.compress_word_def, fpValTreeTheory.fp_bop_def]
+    \\ EVAL_TAC
+    \\ fs[dmode_def, fp64_add_def, fp64_sub_def, fp64mul_def, fp64_div_def]
+    \\ qpat_x_assum ‘float_is_zero (fp64_to_float v1)’ (fn thm => assume_tac (SIMP_RULE std_ss [binary_ieeeTheory.float_is_zero] thm) \\ assume_tac thm)
+    \\ qpat_x_assum ‘float_is_zero (fp64_to_float c)’ (fn thm => assume_tac (SIMP_RULE std_ss [binary_ieeeTheory.float_is_zero] thm) \\ assume_tac thm)
+    \\ fs[binary_ieeeTheory.float_is_zero_def, binary_ieeeTheory.float_add_def]
+    \\ Cases_on ‘float_value (fp64_to_float c)’
+    \\ Cases_on ‘float_value (fp64_to_float v1)’
+    \\ fs[]
+    \\ Cases_on ‘float_value (fp64_to_float c')’ \\ fs[fp64_to_float_float_to_fp64] \\ rveq
+    \\ cheat
+
+Theorem CakeML_FloVer_float_sim:
+  ∀ varMap freshId f theIds freshId2 theCmd E env fVars st vF Gamma.
+  toFloVerCmd varMap freshId f = SOME (theIds, freshId2, theCmd) ∧
+  ids_unique varMap freshId ∧
+  (∀ x m. Gamma x = SOME m ⇒ m = M64) ∧
+  (∀ x y. (x,y) IN fVars ⇒ lookupCMLVar x varMap = SOME (x,y)) ∧
+  env_sim env.v E fVars Gamma ∧
+  (∀ x. x IN freevars [f] ⇒ ∃ y. lookupCMLVar x varMap = SOME (x,y) ∧ (x,y) IN fVars) ∧
+  bstep_float theCmd
+    (λ x. case E x of NONE => NONE | SOME v => SOME (float_to_fp64 (round roundTiesToEven v))) =
+    SOME vF ⇒
+  ∃ st2. evaluate st env [toRealExp f] = (st2, Rval [FP_WordTree (Fp_const vF)])
+Proof
+  cheat
 QED
 
 Theorem CakeML_FloVer_infer_error:
@@ -521,16 +825,16 @@ Theorem CakeML_FloVer_infer_error:
   (∀ x. x IN freevars [f] ⇒ x IN freevars [cake_P]) ∧
   st.fp_state.canOpt = FPScope NoOpt ∧
   (* the free variables are paired up in the id list, and defined *)
-  env_sim env.v E fVars ∧
+  env_sim env.v E fVars (toRExpMap Gamma) ∧
   (∀ x. x IN freevars [cake_P] ⇔ x IN freevars [f]) (* TODO: Should this be checked? *) ∧
   (∀ x. x IN freevars [cake_P] ⇒ ∃ y. lookupCMLVar x varMap = SOME (x,y) ∧ (x,y) IN fVars) ==>
-  ? ids iv err w r.
+  ∃ ids iv err st3 w st4 r.
     (* the analysis result returned contains an error bound *)
     FloverMapTree_find (getRetExp (toRCmd theCmd)) analysisResult = SOME (iv,err) /\
     (* we can evaluate with a real-valued semantics *)
-    evaluate st env [toRealExp f] = (st2, Rval [Real r]) /\
+    evaluate st env [toRealExp f] = (st3, Rval [Real r]) /\
     (* the CakeML code returns a valid floating-point word *)
-    evaluate st env [f] = (st2, Rval [FP_WordTree w]) /\
+    evaluate st env [f] = (st4, Rval [FP_WordTree w]) /\
     (* the roundoff error is sound *)
     real$abs (fp64_to_real (compress_word w) - r)
       <= err
@@ -543,15 +847,39 @@ Proof
   \\ simp[computeErrorbounds_def]
   \\ ntac 4 (TOP_CASE_TAC \\ fs[])
   \\ rpt strip_tac \\ fs[] \\ rveq
+  \\ imp_res_tac CertificateCheckerCmd_Gamma_is_getValidMapCmd
+  \\ fs[] \\ rveq
   \\ imp_res_tac IEEE_connectionTheory.IEEE_connection_cmds
   (* Issue 1: We need to somehow disallow underflow here... *)
   \\ first_x_assum
      (qspecl_then
-      [ ‘λ x. case E x of |SOME v => SOME (real_to_fp64 roundTiesToEven v) | NONE => NONE’,
+      [ ‘λ x. case E x of |SOME v => SOME (float_to_fp64 (round roundTiesToEven v)) | NONE => NONE’,
         ‘E’]
       mp_tac)
   \\ impl_tac
-  >- (cheat)
+  >- (
+    irule approxEnv_construct \\ rpt conj_tac
+    (* Assumption that we do not run into subnormal nums *)
+    >- (cheat)
+    (* assumption from env simulation *)
+    >- (cheat)
+    (* assumption from env simulation ? *)
+    >- (cheat)
+    (* invariant of construction of Gamma *)
+    \\ rpt strip_tac
+    \\ rename1 ‘y IN domain (freeVars (toRCmd theCmd))’
+    \\ ‘y IN domain (freeVars theCmd)’ by fs[toRCmd_freeVars_agree]
+    \\ simp[ExpressionAbbrevsTheory.toRExpMap_def]
+    \\ qspec_then ‘floverVars’ assume_tac is64BitEnv_prepareGamma
+    \\ fs[is64BitEnv_def]
+    \\ imp_res_tac getValidMapCmd_preserving
+    \\ cheat) (* TODO *)
+       (*
+    \\ irule getValidMapCmd_is_64Bit
+
+    \\ asm_exists_tac \\ fs[]
+    \\ qexists_tac ‘FloverMapTree_empty’ \\ fs[FloverMapTree_empty_def, is64BitEnv_def, FloverMapTree_find_def]
+    \\ asm_exists_tac \\ fs[]) *)
   (* TODO: Should this be free vars + domain of Precondition/function parameters? *)
   \\ disch_then (qspec_then ‘freeVars (toRCmd theCmd)’ mp_tac)
   \\ impl_tac \\ fs[]
@@ -560,15 +888,24 @@ Proof
     simp[RealRangeArithTheory.fVars_P_sound_def]
     \\ rpt strip_tac
     \\ first_x_assum irule \\ fs[PULL_EXISTS]
-    \\ qexists_tac ‘[cake_P]’ \\ fs[]
-    \\ qexists_tac ‘env’ \\ rewrite_tac [CONJ_ASSOC]
+    \\ qexists_tac ‘toRExpMap (prepareGamma floverVars)’ \\ qexists_tac  ‘[cake_P]’ \\ fs[]
+    \\ qexists_tac ‘env’
+    \\ rewrite_tac [CONJ_ASSOC]
     \\ once_rewrite_tac [CONJ_COMM]
     \\ asm_exists_tac \\ fs[]
     \\ qexists_tac ‘st’ \\ qexists_tac ‘st2’ \\ fs[]
-    (* Connection between freeVars theCmd and freeVars toRCmd *)
-    \\ ‘v IN domain (freeVars theCmd)’ by (cheat)
-    (* Conclusion: Follows because freevars of CakeML and FloVer program must agree!*)
-    \\ cheat)
+    \\ imp_res_tac toRCmd_freeVars_agree
+    \\ drule toFloVerCmd_freevars_agree \\ fs[]
+    \\ disch_then imp_res_tac \\ fs[]
+    \\ ‘x' IN freevars [cake_P]’ by fs[]
+    \\ first_x_assum (qspec_then ‘x'’ assume_tac)
+    \\ res_tac
+    \\ ‘lookupFloVerVar y varMap = SOME (x', y)’ by fs[ids_unique_def]
+    \\ imp_res_tac toFloVerCmd_lookup_mono
+    \\ ‘lookupFloVerVar y theIds = SOME (x', y)’ by fs[ids_unique_def]
+    \\ imp_res_tac toFloVerCmd_ids_unique
+    \\ ‘y = v’ by (fs[ids_unique_def])
+    \\ rveq \\ fs[])
   \\ impl_tac
   (* Can only be done once we know which environment to pick for the subnormal evaluation*)
   >- (cheat) (* TODO: bstep_valid *)
@@ -587,11 +924,20 @@ Proof
     \\ asm_exists_tac \\ fs[])
   \\ disch_then assume_tac \\ fs[]
   (* Simulation 1: We can get the same result as the FloVer reals from CakeML reals *)
-  \\ ‘evaluate st env [toRealExp f] = (st2, Rval [Real vR'])’
-     by (cheat)
+  \\ ‘∃ st3. evaluate st env [toRealExp f] = (st3, Rval [Real vR'])’
+     by (cheat) (* TODO: Change assumptions *)
+     (* by (drule CakeML_FloVer_real_sim
+         \\ disch_then drule
+         \\ disch_then (qspecl_then [‘st’, ‘a’, ‘vR'’] mp_tac)
+         \\ impl_tac \\ fs[]) *)
   (* Simulation 2: We can get the same result as FloVer floats for CakeML *)
   \\ ‘evaluate st env [f] = (st2, Rval [FP_WordTree (Fp_const vF)])’
-     by (cheat)
+     by (cheat) (* TODO: Change assumptions *)
+        (*
+     by (drule CakeML_FloVer_float_sim
+         \\ disch_then drule
+         \\ disch_then (qspecl_then [‘st’, ‘vF’] mp_tac)
+         \\ impl_tac \\ fs[]) *)
   \\ fsrw_tac [SATISFY_ss] [fpSemTheory.compress_word_def]
   \\ once_rewrite_tac [ABS_SUB]
   \\ simp[fp64_to_real_def]
