icing/CakeMLtoFloVerLemsScript.sml
@@ -1,0 +1,483 @@
+(* HOL4 *)
+open machine_ieeeTheory realTheory realLib RealArith;
+(* CakeML *)
+open compilerTheory;
+(* FloVer *)
+open ExpressionsTheory CommandsTheory IEEE_connectionTheory;
+(* Icing *)
+open CakeMLtoFloVerTheory;
+open preamble;
+
+val _ = new_theory "CakeMLtoFloVerLems";
+
+Definition freevars_def:
+  freevars [] = EMPTY ∧
+  freevars [ast$Var n] = { n } ∧
+  freevars [Lit l] = EMPTY ∧
+  freevars [Raise e] = freevars [e] ∧
+  freevars [Handle e pes] =
+    FOLDL (λ vars. λ (p,e). (freevars [e]) ∪ vars) (freevars [e]) pes ∧
+  freevars [Con id es] = freevars es ∧
+  freevars [Fun s e] = freevars [e] DIFF { Short s } ∧
+  freevars [App op es] = freevars es ∧
+  freevars [Log lop e1 e2] = (freevars [e1] ∪ freevars [e2]) ∧
+  freevars [If e1 e2 e3] = (freevars [e1] ∪ freevars [e2] ∪ freevars [e3]) ∧
+  freevars [Mat e pes] =
+    FOLDL (λ vars. λ (p,e). (freevars [e]) ∪ vars) (freevars [e]) pes ∧
+  freevars [Let x e1 e2] =
+    freevars [e1] ∪
+    (freevars [e2] DIFF (case x of | NONE => EMPTY | SOME s => { Short s })) ∧
+  freevars [Letrec fs e] = EMPTY (* TODO *) ∧
+  freevars [Tannot e t] = freevars [e] ∧
+  freevars [Lannot e l] = freevars [e] ∧
+  freevars [FpOptimise opt e] = freevars [e] ∧
+  freevars (e1::es) =
+    freevars [e1] ∪ freevars es
+Termination
+  wf_rel_tac ‘measure exp6_size’ \\ fs[]
+  \\ Induct_on ‘pes’ \\ fs[]
+  \\ rpt strip_tac \\ simp[astTheory.exp_size_def]  \\ rveq
+  \\ res_tac
+  >- (simp[astTheory.exp_size_def])
+  \\ first_x_assum (qspec_then ‘e’ assume_tac) \\ fs[]
+End
+
+Theorem toFloVerExp_App_cases:
+  ∀ varMap freshId op exps theIds1 freshId1 fexp.
+    toFloVerExp varMap freshId (App op exps) = SOME (theIds1, freshId1, fexp) ⇒
+    (∃ e fexp2.
+       (op = FP_uop FP_Neg ∧ exps = [e] ∧
+       toFloVerExp varMap freshId e = SOME (theIds1, freshId1, fexp2) ∧
+       fexp = Unop Neg fexp2)) ∨
+    (∃ e1 e2 bop theIds2 freshId2 fexp1 fexp2.
+      (op = FP_bop bop ∧ exps = [e1; e2] ∧
+       toFloVerExp varMap freshId e1 = SOME (theIds2, freshId2, fexp1) ∧
+       toFloVerExp theIds2 freshId2 e2 = SOME (theIds1, freshId1, fexp2) ∧
+       fexp = Binop (fpBopToFloVer bop) fexp1 fexp2)) ∨
+    (∃ e1 e2 e3 theIds2 theIds3 freshId2 freshId3 fexp1 fexp2 fexp3.
+      (op = FP_top FP_Fma ∧ exps = [e1; e2; e3] ∧
+       toFloVerExp varMap freshId e1 = SOME (theIds2, freshId2, fexp1) ∧
+       toFloVerExp theIds2 freshId2 e2 = SOME (theIds3, freshId3, fexp2) ∧
+       toFloVerExp theIds3 freshId3 e3 = SOME (theIds1, freshId1, fexp3) ∧
+       fexp = Fma fexp1 fexp2 fexp3))
+Proof
+  fs[toFloVerExp_def, option_case_eq, list_case_eq]
+  \\ Cases_on ‘op’ \\ fs[]
+  \\ TRY (Cases_on ‘f’)
+  \\ fs[list_case_eq, option_case_eq, pair_case_eq]
+  \\ rpt strip_tac \\ fs[] \\ rveq \\ fs[]
+QED
+
+Theorem toFloVerExp_usedVars:
+  ∀ ids freshId e ids2 freshId2 fexp.
+    toFloVerExp ids freshId e = SOME (ids2, freshId2, fexp) ⇒
+    ∀ n. freshId ≤ n ∧ n < freshId2 ⇒
+      n IN domain (usedVars (fexp))
+Proof
+  ho_match_mp_tac toFloVerExp_ind
+  \\ rpt strip_tac \\ TRY (fs[toFloVerExp_def] \\ NO_TAC)
+  >- (
+   qpat_x_assum ‘_ = SOME _’ mp_tac \\ fs[toFloVerExp_def]
+   \\ rpt (TOP_CASE_TAC \\ fs[])
+   \\ rpt strip_tac \\ rveq \\ fs[usedVars_def])
+  \\ first_x_assum (mp_then Any assume_tac toFloVerExp_App_cases)
+  \\ fs[] \\ rveq \\ fs[]
+  \\ simp[Once usedVars_def, domain_union]
+  \\ TRY (metis_tac[])
+  \\ TRY (Cases_on ‘n < freshId2'’\\ fs[] \\ metis_tac[])
+  \\ TRY (Cases_on ‘n < freshId2'’\\ fs[] \\ TRY (metis_tac[])
+          \\ Cases_on ‘n < freshId3’ \\ fs[] \\ metis_tac[])
+QED
+
+Theorem lookupCMLVar_id_l:
+  lookupCMLVar x ids = SOME (y, n) ⇒
+  x = y
+Proof
+  Induct_on ‘ids’ \\ fs[lookupCMLVar_def, updateTheory.FIND_def]
+  \\ strip_tac \\ rename1 ‘(λ (m,i). x = m) h’ \\ Cases_on ‘h’ \\  fs[]
+  \\ TOP_CASE_TAC \\ fs[]
+QED
+
+Theorem lookupFloVerVar_id_r:
+  lookupFloVerVar n ids = SOME (x,m) ⇒
+  n = m
+Proof
+  Induct_on ‘ids’ \\ fs[lookupFloVerVar_def, updateTheory.FIND_def]
+  \\ strip_tac \\ rename1 ‘(λ (m,i). n = i) h’ \\ Cases_on ‘h’ \\  fs[]
+  \\ TOP_CASE_TAC \\ fs[]
+QED
+
+Theorem getInterval_inv:
+  getInterval e = SOME (x,lo,hi) ⇒
+  freevars [e] = { Short x } ∧
+  ∃ w1 w2.
+  e = Log And (App (FP_cmp FP_LessEqual) [Lit (Word64 w1); Var (Short x)])
+  (App (FP_cmp FP_LessEqual) [Var (Short x); Lit (Word64 w2)]) ∧
+  lo = fp64_to_real w1 ∧
+  hi = fp64_to_real w2 ∧
+  fp64_isFinite w1 ∧
+  fp64_isFinite w2
+Proof
+  Cases_on ‘e’ \\ simp[getInterval_def]
+  \\ rpt (TOP_CASE_TAC \\ fs[])
+  \\ rpt strip_tac \\ rveq \\ fs[freevars_def]
+QED
+
+Theorem toFloVerPre_freevar_FIND:
+  ∀ cake_P ids floverP dVars.
+  toFloVerPre cake_P ids = SOME (floverP, dVars) ⇒
+  ∀ x. x IN freevars cake_P ⇒
+  ∃ n m. lookupCMLVar x ids = SOME (x, n) ∧
+  FIND (λ m. n = m) dVars = SOME m
+Proof
+  ho_match_mp_tac toFloVerPre_ind
+  \\ rpt strip_tac \\ fs[toFloVerPre_def]
+  \\ qpat_x_assum ‘_ = SOME (_, _)’ mp_tac
+  \\ reverse TOP_CASE_TAC \\ fs[]
+  >- (
+    rpt (TOP_CASE_TAC \\ fs[])
+    \\ first_assum (mp_then Any assume_tac getInterval_inv)
+    \\ rpt strip_tac \\ fs[] \\ rveq
+    \\ first_assum (mp_then Any assume_tac lookupCMLVar_id_l)
+    \\ rveq \\ fsrw_tac [SATISFY_ss] [updateTheory.FIND_def])
+  \\ rpt (TOP_CASE_TAC \\ fs[])
+  \\ rpt strip_tac \\ rveq
+  \\ fs[freevars_def]
+  >- (
+    first_assum (mp_then Any assume_tac getInterval_inv)
+    \\ first_assum (mp_then Any assume_tac lookupCMLVar_id_l)
+    \\ fs[] \\ rveq
+    \\ fsrw_tac [SATISFY_ss] [updateTheory.FIND_def])
+  \\ res_tac
+  \\ imp_res_tac lookupCMLVar_id_l \\ rveq
+  \\ fsrw_tac [SATISFY_ss] [updateTheory.FIND_def]
+  \\ TOP_CASE_TAC \\ fs[]
+QED
+
+Definition ids_unique_def:
+  ids_unique ids (freshId:num) =
+  ((∀ x y z.
+    lookupCMLVar x ids = SOME (x, y) ∧
+    lookupFloVerVar z ids = SOME (x, z) ⇒
+    z = y) ∧
+  (∀ x y z.
+    lookupCMLVar (Short x) ids = SOME (Short x, z) ∧
+    lookupFloVerVar z ids = SOME (Short y, z) ⇒
+    x = y) ∧
+  (∀ x y z.
+    lookupCMLVar x ids = SOME (x,z) ∧
+    lookupCMLVar y ids = SOME (y,z) ⇒
+    x = y) ∧
+  (∀ x y z.
+    lookupFloVerVar x ids = SOME (z,x) ∧
+    lookupFloVerVar y ids = SOME (z,y) ⇒
+    x = y) ∧
+  (∀ x y.
+    lookupFloVerVar x ids = SOME (y, x) ⇒
+    lookupCMLVar y ids = SOME (y,x)) ∧
+  (∀ x y.
+    lookupCMLVar y ids = SOME (y,x) ⇒
+    lookupFloVerVar x ids = SOME (y, x)) ∧
+  (∀ id. freshId ≤ id ⇒ lookupFloVerVar id ids = NONE) ∧
+  (∀ x y. lookupCMLVar x ids = SOME (x, y) ⇒
+     y < freshId))
+End
+
+Theorem prepareVars_is_unique:
+  ∀ ids floverVars varMap freshId.
+    prepareVars ids = (floverVars, varMap, freshId) ⇒
+    ids_unique varMap freshId
+Proof
+  Induct_on ‘ids’ \\ fs[prepareVars_def]
+  >- (
+    rpt strip_tac \\ fs[] \\ rveq
+    \\ fs[ids_unique_def, lookupCMLVar_def, lookupFloVerVar_def,
+          updateTheory.FIND_def])
+  \\ Cases_on ‘prepareVars ids’ \\ rename1 ‘prepareVars ids = (floverVars, p)’
+  \\ Cases_on ‘p’ \\ rename1 ‘prepareVars ids = (floverVars, varMap, freshId)’
+  \\ fs[ids_unique_def] \\ rpt strip_tac \\ rpt conj_tac
+  \\ fs[appendCMLVar_def]
+  \\ Cases_on ‘lookupCMLVar (Short h) varMap’
+  \\ fs[lookupCMLVar_def, lookupFloVerVar_def, updateTheory.FIND_def]
+  \\ every_case_tac \\ rveq \\ fs[]
+  \\ res_tac \\ rveq \\ fs[]
+QED
+
+Theorem toFloVerExp_noDowncast:
+  ∀ varMap freshId e theIds freshId2 theExp.
+    toFloVerExp varMap freshId e = SOME (theIds, freshId2, theExp) ⇒
+    noDowncast (toRExp theExp)
+Proof
+  ho_match_mp_tac toFloVerExp_ind
+  \\ rpt strip_tac \\ fs[toFloVerExp_def, toRExp_def, noDowncast_def]
+  \\ rveq \\ fs[toRExp_def, noDowncast_def]
+  \\ every_case_tac \\ fs[] \\ rveq
+  \\ fs[toRExp_def, noDowncast_def]
+QED
+
+Theorem toFloVerCmd_noDowncastFun:
+  ∀ varMap freshId f theIds freshId2 theCmd.
+    toFloVerCmd varMap freshId f = SOME (theIds, freshId2, theCmd) ⇒
+    noDowncastFun (toRCmd theCmd)
+Proof
+  ho_match_mp_tac toFloVerCmd_ind
+  \\ rpt strip_tac \\ fs[toFloVerCmd_def, toRCmd_def, noDowncastFun_def]
+  \\ every_case_tac \\ fs[toRCmd_def, noDowncastFun_def] \\ rveq
+  \\ fs[toRCmd_def, noDowncastFun_def]
+  \\ irule toFloVerExp_noDowncast \\ asm_exists_tac \\ fs[]
+QED
+
+Theorem is64BitEnv_prepareGamma:
+  ∀ floverVars. is64BitEnv (prepareGamma floverVars)
+Proof
+  Induct_on ‘floverVars’ \\ fs[is64BitEnv_def, prepareGamma_def]
+  >- (
+   rpt strip_tac
+   \\ fs[FloverMapTheory.FloverMapTree_find_def,
+         FloverMapTheory.FloverMapTree_empty_def])
+  \\ rpt strip_tac \\ fs[FloverMapTheory.map_find_add]
+  \\ every_case_tac \\ fs[] \\ res_tac
+QED
+
+Theorem toFloVerExp_is64BitEval:
+  ∀ varMap freshId e theIds freshId2 theExp.
+    toFloVerExp varMap freshId e = SOME (theIds, freshId2, theExp) ⇒
+    is64BitEval (toRExp theExp)
+Proof
+  ho_match_mp_tac toFloVerExp_ind
+  \\ rpt strip_tac \\ fs[toFloVerExp_def, toRExp_def, is64BitEval_def]
+  \\ rveq \\ fs[toRExp_def, is64BitEval_def]
+  \\ every_case_tac \\ fs[] \\ rveq
+  \\ fs[toRExp_def, is64BitEval_def]
+QED
+
+Theorem toFloVerCmd_is64BitBstep:
+  ∀ varMap freshId f theIds freshId2 theCmd.
+    toFloVerCmd varMap freshId f = SOME (theIds, freshId2, theCmd) ⇒
+    is64BitBstep (toRCmd theCmd)
+Proof
+  ho_match_mp_tac toFloVerCmd_ind
+  \\ rpt strip_tac \\ fs[toFloVerCmd_def, toRCmd_def, is64BitBstep_def]
+  \\ every_case_tac \\ fs[toRCmd_def, is64BitBstep_def] \\ rveq
+  \\ fs[toRCmd_def, is64BitBstep_def]
+  \\ irule toFloVerExp_is64BitEval \\ asm_exists_tac \\ fs[]
+QED
+
+Theorem lookupCMLVar_appendCMLVar:
+  ∀ x y freshId varMap.
+    lookupCMLVar x (appendCMLVar y freshId varMap) =
+    case lookupCMLVar y varMap of
+    | NONE => lookupCMLVar x ((y,freshId)::varMap)
+    | SOME _ => lookupCMLVar x varMap
+Proof
+  rpt strip_tac \\ fs[appendCMLVar_def]
+  \\ TOP_CASE_TAC \\ fs[lookupCMLVar_def, updateTheory.FIND_def]
+QED
+
+Theorem lookupFloVerVar_appendCMLVar:
+  ∀ x y freshId varMap.
+    lookupFloVerVar x (appendCMLVar y freshId varMap) =
+    case lookupCMLVar y varMap of
+    | NONE => lookupFloVerVar x ((y, freshId)::varMap)
+    | SOME _ => lookupFloVerVar x varMap
+Proof
+  rpt strip_tac \\ fs[appendCMLVar_def]
+  \\ TOP_CASE_TAC \\ fs[lookupFloVerVar_def, updateTheory.FIND_def]
+QED
+
+Theorem ids_unique_append:
+  ∀ x varMap freshId.
+    ids_unique varMap freshId ⇒
+    ids_unique (appendCMLVar x freshId varMap) (freshId + 1)
+Proof
+  rpt strip_tac \\ fs[ids_unique_def]
+  \\ rpt conj_tac \\ rpt strip_tac \\ fs[] \\ res_tac
+  \\ fs[lookupCMLVar_appendCMLVar, lookupFloVerVar_appendCMLVar]
+  \\ every_case_tac \\ fs[lookupFloVerVar_def, lookupCMLVar_def, updateTheory.FIND_def]
+  \\ every_case_tac \\ rveq \\ fs[] \\ res_tac \\ fs[]
+QED
+
+Theorem toFloVerExp_ids_unique:
+  ∀ varMap freshId f theIds freshId2 theExp.
+    toFloVerExp varMap freshId f = SOME (theIds, freshId2, theExp) ∧
+    ids_unique varMap freshId ⇒
+    ids_unique theIds freshId2
+Proof
+  ho_match_mp_tac toFloVerExp_ind
+  \\ rpt strip_tac
+  \\ fs[Once toFloVerExp_def, option_case_eq, pair_case_eq, list_case_eq]
+  \\ rveq \\ fs[ids_unique_append]
+  \\ Cases_on ‘op’ \\ fs[list_case_eq, option_case_eq, pair_case_eq] \\ rveq
+  \\ Cases_on ‘f’ \\ fs[option_case_eq, pair_case_eq]
+QED
+
+Theorem toFloVerCmd_ids_unique:
+  ∀ varMap freshId f theIds freshId2 theCmd.
+    toFloVerCmd varMap freshId f = SOME (theIds, freshId2, theCmd) ⇒
+    ids_unique varMap freshId ⇒
+    ids_unique theIds freshId2
+Proof
+  ho_match_mp_tac toFloVerCmd_ind
+  \\ rpt strip_tac
+  \\ fs[Once toFloVerCmd_def, option_case_eq, pair_case_eq] \\ rveq
+  \\ fs[]
+  \\ imp_res_tac toFloVerExp_ids_unique
+  \\ imp_res_tac ids_unique_append
+  \\ fs[]
+QED
+
+Theorem toFloVerExp_lookup_mono:
+  ∀ ids freshId e ids2 freshId2 fexp.
+  toFloVerExp ids freshId e = SOME (ids2, freshId2, fexp) ⇒
+  ids_unique ids freshId ⇒
+  (∀ n x. lookupFloVerVar n ids = SOME (x, n) ⇒
+   lookupFloVerVar n ids2 = SOME (x,n)) ∧
+  (∀ x n. lookupCMLVar x ids = SOME (x,n) ⇒
+   lookupCMLVar x ids2 = SOME (x,n))
+Proof
+  ho_match_mp_tac toFloVerExp_ind
+  \\ rpt strip_tac
+  \\ ((rename1 ‘App op exps’ \\ imp_res_tac toFloVerExp_App_cases)
+     ORELSE
+     (qpat_x_assum ‘toFloVerExp _ _ _ = SOME _’ mp_tac
+      \\ simp[Once toFloVerExp_def] \\ rpt strip_tac))
+  >- (
+    fs[option_case_eq, pair_case_eq] \\ rveq
+    \\ fs[lookupFloVerVar_appendCMLVar, lookupFloVerVar_def, ids_unique_def, updateTheory.FIND_def]
+    \\ TOP_CASE_TAC \\ fs[] \\ rveq \\ first_x_assum (qspec_then ‘freshId’ assume_tac) \\ fs[])
+  >- (
+    fs[option_case_eq, pair_case_eq] \\ rveq
+    \\ fs[lookupCMLVar_appendCMLVar, lookupCMLVar_def, ids_unique_def, updateTheory.FIND_def]
+    \\ TOP_CASE_TAC \\ fs[] \\ rveq \\ first_x_assum (qspec_then ‘freshId’ assume_tac) \\ fs[])
+  >- (
+     rveq \\ fs[])
+  >- (
+     rveq \\ fs[])
+  \\ rveq \\ fs[] \\ rpt strip_tac \\ TRY (Cases_on ‘f’) \\ fs[option_case_eq, pair_case_eq]
+  \\ rveq \\ imp_res_tac toFloVerExp_ids_unique
+  \\ res_tac \\ res_tac
+QED
+
+Theorem toFloVerCmd_lookup_mono:
+  ∀ ids freshId e ids2 freshId2 theCmd.
+  toFloVerCmd ids freshId e = SOME (ids2, freshId2, theCmd) ⇒
+  ids_unique ids freshId ⇒
+  (∀ n x. lookupFloVerVar n ids = SOME (x, n) ⇒
+   lookupFloVerVar n ids2 = SOME (x,n)) ∧
+  (∀ x n. lookupCMLVar x ids = SOME (x,n) ⇒
+   lookupCMLVar x ids2 = SOME (x,n))
+Proof
+  ho_match_mp_tac toFloVerCmd_ind
+  \\ rpt strip_tac
+  \\ qpat_x_assum ‘toFloVerCmd _ _ _ = SOME _’ mp_tac
+  \\ simp[Once toFloVerCmd_def] \\ rpt strip_tac
+  \\ TRY (fs[option_case_eq, pair_case_eq] \\ rveq \\ imp_res_tac toFloVerExp_lookup_mono)
+  \\ fs[]
+  \\ last_x_assum mp_tac \\ impl_tac \\ fs[]
+  \\ TRY (irule ids_unique_append \\ irule toFloVerExp_ids_unique \\ asm_exists_tac \\ fs[])
+  \\ strip_tac
+  \\ first_x_assum irule
+  \\ fs[lookupFloVerVar_appendCMLVar, lookupCMLVar_appendCMLVar,
+        lookupFloVerVar_def, lookupCMLVar_def, updateTheory.FIND_def]
+  \\ TOP_CASE_TAC \\ fs[] \\ rveq
+  \\ imp_res_tac toFloVerExp_ids_unique
+  \\ fs[ids_unique_def] \\ fs[lookupFloVerVar_def, lookupCMLVar_def]
+QED
+
+Theorem toFloVerExp_freevars_agree:
+  ∀ varMap freshId f theIds freshId2 theExp v.
+    toFloVerExp varMap freshId f = SOME (theIds, freshId2, theExp) ∧
+    ids_unique varMap freshId ∧
+    v ∈ domain (usedVars theExp) ⇒
+    ∃ x. lookupFloVerVar v theIds = SOME (x, v) ∧
+      x IN freevars [f]
+Proof
+  ho_match_mp_tac toFloVerExp_ind
+  \\ rpt strip_tac
+  \\ fs[Once toFloVerExp_def, option_case_eq, pair_case_eq, list_case_eq]
+  \\ rveq
+  >- (
+    fs[usedVars_def, freevars_def] \\ rveq
+    \\ fs[lookupFloVerVar_def, appendCMLVar_def, updateTheory.FIND_def])
+  >- (
+    fs[usedVars_def, freevars_def] \\ rveq \\ fs[ids_unique_def]
+    \\ imp_res_tac lookupCMLVar_id_l \\ rveq
+    \\ res_tac \\ fs[])
+  >- (
+    fs[usedVars_def])
+  \\ Cases_on ‘op’ \\ fs[list_case_eq, option_case_eq] \\ rveq
+  \\ TRY (Cases_on ‘f’) \\ fs[option_case_eq, pair_case_eq]
+  \\ rveq \\ qpat_x_assum ‘_ IN domain (usedVars _)’ mp_tac
+  \\ simp[Once usedVars_def, domain_union] \\ rpt strip_tac
+  \\ imp_res_tac toFloVerExp_ids_unique
+  \\ TRY (fs[] \\ res_tac \\ fsrw_tac [SATISFY_ss] [freevars_def])
+  \\ imp_res_tac toFloVerExp_lookup_mono
+  \\ res_tac \\ fs[]
+QED
+
+Theorem toFloVerCmd_freevars_agree:
+  ∀ varMap freshId f theIds freshId2 theCmd v.
+    toFloVerCmd varMap freshId f = SOME (theIds, freshId2, theCmd) ∧
+    ids_unique varMap freshId ∧
+    v ∈ domain (freeVars theCmd) ⇒
+    ∃ x. lookupFloVerVar v theIds = SOME (x, v) ∧
+      x IN freevars [f]
+Proof
+  ho_match_mp_tac toFloVerCmd_ind
+  \\ rpt strip_tac
+  \\ fs[Once toFloVerCmd_def, option_case_eq, pair_case_eq] \\ rveq
+  \\ TRY (fs[Once freeVars_def] \\ imp_res_tac toFloVerExp_freevars_agree \\ fs[] \\ NO_TAC)
+  \\ fs[]
+  \\ imp_res_tac toFloVerExp_ids_unique
+  \\ imp_res_tac toFloVerCmd_ids_unique
+  \\ qpat_x_assum ‘v IN domain (freeVars _)’ mp_tac
+  \\ rename1 ‘ids_unique (appendCMLVar (Short x) freshId3 ids2) (freshId3 + 1)’
+  \\ ‘ids_unique (appendCMLVar (Short x) freshId3 ids2) (freshId3 + 1)’
+     by (irule ids_unique_append \\ fs[])
+  \\ fs[]
+  \\ simp[Once freeVars_def, domain_union] \\ rpt strip_tac \\ fs[]
+  >- (
+    imp_res_tac toFloVerExp_freevars_agree \\ fs[] \\ rveq
+    \\ imp_res_tac toFloVerCmd_lookup_mono \\ fs[]
+    \\ rename1 ‘lookupFloVerVar n ids2 = SOME (y,n)’
+    \\ ‘lookupFloVerVar n (appendCMLVar (Short x) freshId3 ids2) = SOME (y,n)’
+      by (fs[lookupFloVerVar_appendCMLVar, lookupFloVerVar_def,
+             updateTheory.FIND_def])
+    \\ res_tac \\ fs[freevars_def])
+  \\ first_x_assum drule \\ fs[freevars_def] \\ disch_then assume_tac
+  \\ fs[]
+  \\ Cases_on ‘x' = Short x’ \\ fs[]
+  \\ rveq
+  \\ ‘lookupCMLVar (Short x) ids3 = SOME (Short x, v)’
+    by (fs[ids_unique_def])
+  \\ fs[appendCMLVar_def]
+  \\ ‘lookupCMLVar (Short x) ((Short x, freshId3)::ids2) = SOME (Short x, freshId3)’
+     by EVAL_TAC
+  \\ rfs[]
+  \\ imp_res_tac toFloVerCmd_lookup_mono
+  \\ fs[]
+QED
+
+Theorem toRExp_usedVars_agree:
+  ∀ v e.
+    v IN (domain (usedVars (toRExp e))) ⇒
+    v IN domain (usedVars e)
+Proof
+  Induct_on ‘e’ \\ simp[Once usedVars_def, toRExp_def, domain_union]
+  \\ rpt strip_tac \\ res_tac
+  \\ simp[Once usedVars_def, domain_union]
+QED
+
+Theorem toRCmd_freeVars_agree:
+  ∀ v theCmd.
+  v IN (domain (freeVars (toRCmd theCmd))) ⇒
+  v IN domain (freeVars theCmd)
+Proof
+  Induct_on ‘theCmd’ \\ simp[Once freeVars_def, toRCmd_def, domain_union]
+  \\ rpt strip_tac
+  \\ imp_res_tac toRExp_usedVars_agree
+  \\ res_tac
+  \\ simp[Once freeVars_def, domain_union]
+QED
+
+val _ = export_theory();
